---
title: Ex. 13.3
linktitle: Ex 13.3
type: book
date: "2021-01-02T00:00:00+01:00"
# Prev/next pager order (if `docs_section_pager` enabled in `params.toml`)
weight: 1
toc: false
---

???+ question "Ex. 13.3"
    Let $E^\ast$ be the error rate of the Bayes rule in a $K$-class problem, where the true class probabilities are given by $p_k(x)$, $k=1,...,K$. Assuming the test point and training point have identical features $x$, prove (13.5)
	
    \begin{equation}
		\sum_{k=1}^Kp_k(x)(1-p_k(x)) \le 2(1-p_{k^\ast}(x))-\frac{K}{K-1}(1-p_{k^\ast}(x))^2,\non
	\end{equation}
	
    where $k^\ast = \underset{k}{\operatorname{argmax}}p_k(x)$. Hence argue that the error rate of the 1-nearest-neighbor rule converge in $L_1$, as the size of the training set increases, to a value $E_1$, bounded above by
	
    \begin{equation}
		E^\ast\left(2-E^\ast\frac{K}{K-1}\right).\non
	\end{equation}
	
    [This statement of the theorem of \cite{cover1967nearest} is taken from Chapter 6 of \cite{ripley1996pattern}, where a short proof is also given].

??? done "Soln. 13.3"
	We write 
	
    \begin{equation}
		\sum_{k=1}^Kp_k(x)(1-p_k(x)) = 1 -\sum_{k=1}^Kp_k(x)^2 = 1-p_{k^\ast}(x)^2 - \sum_{i\neq k^\ast}^K p_i(x)^2,\non
	\end{equation}
	
    and we need to minimize $\sum_{i\neq k^\ast}^K p_i(x)^2$. It's easy to see (consider its Lagrangian) that it's minimized when each $p_i(x)$ for $i\neq k^\ast$ are equal. With the constraint that $\sum_{i=1}^Kp_i(x)=1$, we get $p_i(x) = \frac{1}{K-1}(1-p_{k^\ast}(x))$ for $i\neq k^\ast$. Plug it into the equation with simple algebra we obtain
	
    \begin{eqnarray}
		\sum_{k=1}^Kp_k(x)(1-p_k(x)) &\le& 1-p_{k^\ast}(x)^2 - (K-1)\left(\frac{1}{K-1}(1-p_{k^\ast}(x))\right)^2\non\\
		&=&1-p_{k^\ast}(x)^2 - \frac{(1-p_{k^\ast}(x))^2}{K-1}\non\\
		%&=&1-p_{k^\ast}(x)^2 + (1-p_{k^\ast}(x))^2 - (1-p_{k^\ast}(x))^2 - \frac{(1-p_{k^\ast}(x))^2}{K-1}\non\\
		&=&2(1-p_{k^\ast}(x)) - \frac{K}{K-1}(1-p_{k^\ast}(x))^2.\label{eq:13-3b}
	\end{eqnarray}

	By definition we have
	
    \begin{equation}
		E_1 = \int \left[\sum_{k=1}^Kp_k(x)(1-p_k(x))\right]p(x)dx\non
	\end{equation}
	
    and 
	
    \begin{equation}
		E^\ast = \int \left[1-p_{k^\ast}(x)\right]p(x)dx.\non
	\end{equation}
	
    Therefore, by $\eqref{eq:13-3b}$ we obtain

	\begin{equation}
		E_1 \le E^\ast\left(2-E^\ast\frac{K}{K-1}\right).\non
	\end{equation}
    