---
title: Ex. 18.20
linktitle: Ex 18.20
---

???+ question "Ex. 18.20"
	*Proof of result (18.53)*. Write 
	
    \begin{eqnarray}
		\text{pFDR} &=& E\left(\frac{V}{R}|R > 0\right)\non\\
		&=&\sum_{k=1}^ME\left[\frac{V}{R}|R=k\right]\text{Pr}(R=k|R > 0)\non
	\end{eqnarray}
	
    Use the fact that given $R=k$, $V$ is a binomial random variable, with $k$ trials and probability of success $\text{Pr}(H=0|T\in \Gamma)$, to complete the proof.

??? done "Soln. 18.20"
 	Note that given $R=k$, $V$ is a binomial random variable, with $k$ trials and probability of success $\text{Pr}(H=0|T\in \Gamma)$, we have 
	
    \begin{equation}
		E[V|R=k] = k \cdot \text{Pr}(H=0|T\in \Gamma).\non
	\end{equation}
	
    Therefore, 
	
    \begin{eqnarray}
		\text{pFDR}(\Gamma) &=&\sum_{k=1}^M\frac{1}{k} \cdot k \cdot \text{Pr}(H=0|T\in \Gamma)\text{Pr}(R=k|R > 0)\non\\
		&=&\text{Pr}(H=0|T\in \Gamma)\sum_{k=1}^M\text{Pr}(R=k|R > 0)\non\\
		&=&\text{Pr}(H=0|T\in \Gamma).\non
	\end{eqnarray}

	Note the notation $H$ comes from \cite{storey2003positive}, and it should be $Z$ defined (18.51) in our context.