---
title: Ex. 7.3
linktitle: Ex 7.3
type: book
date: "2021-01-02T00:00:00+01:00"
# Prev/next pager order (if `docs_section_pager` enabled in `params.toml`)
weight: 1
toc: false
---

???+ question "Ex. 7.3"
    Let $\boldsymbol{\hat f} = \bb{S}\bb{y}$ be a linear smoothing of $\bb{y}$.
    ???+ question "(a)"
	    If $S_{ii}$ is the $i$th diagonal element of $\bb{S}$, show that for $\bb{S}$ arising from least squares projections and cubic smoothing splines, the cross-validated residual can be written as 
	    
        \begin{equation}
	    \label{eq:ex73-a}
		y_i - \hat f^{-i}(x_i) = \frac{y_i - \hat f(x_i)}{1-S_{ii}}.
	    \end{equation}

    ???+ question "(b)"
	    Use this result to show that $|y_i-\hat f^{-i}(x_i)| \ge |y_i - \hat f(x_i)|$.

    ???+ question "(c)"
	    Find general conditions on any smoother $\bb{S}$ to make result $\eqref{eq:ex73-a}$ hold.

??? done "Soln. 7.3"
    Without loss of generality, we assume

	\begin{equation}
		\bb{S} = \bb{X}(\bb{X}^T\bb{X} + \lambda \bm{\Omega})^{-1}\bb{X}^T.\non
	\end{equation}

	For least squares we have $\lambda=0$, and for cubic smoothing we have $\lambda\ge 0$. See Chapters 3 & 5 in the text for more details.

    ??? done "(a)"
        We have

        \begin{eqnarray}
            S_{ii} &=& x_i^T(\bb{X}^T\bb{X} + \lambda \bm{\Omega})^{-1}x_i,\non\\
            \hat f(x_i) &=& x_i^T(\bb{X}^T\bb{X} + \lambda \bm{\Omega})^{-1}\bb{X}^T\bb{y}.\non
        \end{eqnarray}

        Let $\bb{X}_{-i}$ and $\bb{y}_{-i}$ be the corresponding results with $x_i$ removed, then we have
        
        \begin{eqnarray}
            \hat f^{-i}(x_i) &=& x_i^T(\bb{X}_{-i}^T\bb{X}_{-i} + \lambda \bm{\Omega})^{-1}\bb{X}_{-i}^T\bb{y}_{-i}\non\\
            &=&x_i^T(\bb{X}^T\bb{X} - x_ix_i^T + \lambda \bm{\Omega})^{-1}(\bb{X}^T\bb{y}-x_iy_i).\label{eq:73-1}
        \end{eqnarray}

        Let $\bb{A} = (\bb{X}^T\bb{X} + \lambda\Omega)$, by [Woodbury matrix identity](https://en.wikipedia.org/wiki/Woodbury_matrix_identity), we have
        
        \begin{eqnarray}
            (\bb{A}-x_ix_i^T)^{-1} &=& \bb{A}^{-1} + \frac{\bb{A}^{-1}x_ix_i^T\bb{A}^{-1}}{1-x_i^T\bb{A}^{-1}x_i}.\non 
        \end{eqnarray}
        
        Therefore, $\eqref{eq:73-1}$ becomes
        
        \begin{eqnarray}
            \hat f^{-1}(x_i) &=& x_i^T\left(\bb{A}^{-1} + \frac{\bb{A}^{-1}x_ix_i^T\bb{A}^{-1}}{1-x_i^T\bb{A}^{-1}x_i}\right)(\bb{X}^T\bb{y}-x_iy_i)\non\\
            &=&\left(x_i^T\bb{A}^{-1} + \frac{S_{ii}x_i^T\bb{A}^{-1}}{1-S_{ii}}\right)(\bb{X}^T\bb{y}-x_iy_i)\non\\
            &=&x_i^T\bb{A}^{-1}\bb{X}^T\bb{y} - x_i^T\bb{A}^{-1}x_iy_i + \frac{S_{ii}x_i^T\bb{A}^{-1}\bb{X}^T\bb{y}}{1-S_{ii}} - \frac{S_{ii}x_i^T\bb{A}^{-1}x_iy_i}{1-S_{ii}}\non\\
            &=&\hat f(x_i) -y_iS_{ii} + \frac{S_{ii}\hat f(x_i)}{1-S_{ii}} - \frac{y_iS_{ii}^2}{1-S_{ii}}\non\\
            &=&\frac{\hat f(x_i) - y_i S_{ii}}{1-S_{ii}}.\non
        \end{eqnarray}
        
        Therefore by simple algebra we have $\eqref{eq:ex73-a}$.
    
    ??? done "(b)"  
        Note that $\bb{S} = \bb{X}(\bb{X}^T\bb{X} + \lambda \bm{\Omega})^{-1}\bb{X}^T$ is positive-semidefinite and has eigen-decomposition 
        
        \begin{equation}
            \bb{S} = \sum_{k=1}^N\rho_k(\lambda)\bb{u}_k\bb{u}_k^T.\non
        \end{equation}

        See Section 5.4.1 in the text for more details. Therefore, we know that $\bb{S}\bb{S} \preceq \bb{S}$, so that

        \begin{equation}
            0\le (S^2)_{ii} = \sum_{k\neq i}S_{ik}^2 + S_{ii}^2\le S_{ii}\non
        \end{equation}
        
        from which we know $0\le S_{ii} \le 1$.

        By $\eqref{eq:ex73-a}$ we have $|y_i-\hat f^{-i}(x_i)| \ge |y_i - \hat f(x_i)|$.

    ??? done "(c)"
        For general linear smoother $\boldsymbol{\hat f} = \bb{S}\bb{y}$, if $\bb{S}$ only depends on $\bb{X}$ and other tuning parameters (i.e., independent of $\bb{y}$), $\eqref{eq:ex73-a}$ still holds.

        To see that, note that if we replace $y_i$ with $\hat f^{-i}(x_i)$ (obtained by \eqref{eq:73-1}) in $\textbf{y}$ and denote the new vector by $\textbf{y}'$, $\textbf{S}$ is not changed. Thus we have
        
        \begin{eqnarray}
            \hat f^{-i}(x_i)
            &=&(\textbf{S}\textbf{y}')_i\non\\
            &=& \sum_{i\neq j}S_{ij}\textbf{y}'_j + S_{ii}\hat f^{-i}(x_i)\non\\
            &=&\hat f(x_i) - S_{ii}y_i + S_{ii}\hat f^{-i}(x_i),\non
        \end{eqnarray}
        
        therefore we obtain $\eqref{eq:ex73-a}$. 