---
title: Ex. 17.6
linktitle: Ex 17.6
type: book
date: "2021-01-02T00:00:00+01:00"
# Prev/next pager order (if `docs_section_pager` enabled in `params.toml`)
weight: 1
toc: false
---

???+ question "Ex. 17.6"
	*Recovery of $\hat{\bm{\Theta}}=\hat{\bm{\Sigma}}^{-1}$ from Algorithm 17.1*. Use expression (17.16) to derive the standard partitioned inverse expressions
	
    \begin{eqnarray}
		\theta_{12} &=& -\bb{W}^{-1}_{11}w_{12}\theta_{22}\non\\
		\theta_{22} &=&1/(w_{22}-w_{12}^T\bb{W}_{11}^{-1}w_{12}).\non
	\end{eqnarray}
	
    Since $\hat\beta = \bb{W}_{11}^{-1}w_{12}$, show that $\hat\theta_{22} = 1/(w_{22}-w_{12}^T\hat\beta)$ and $\hat\theta_{12} = -\hat\beta\hat\theta_{22}$. Thus $\hat\theta_{12}$ is a simply rescaling of $\hat\beta$ by $-\hat\theta_{22}$.

??? done "Soln. 17.6"
	From (17.16) in the text we have
	
    \begin{equation}
		\label{eq:17-6a}
		\theta_{12} = -\bb{W}^{-1}_{11}w_{12}\theta_{22}.
	\end{equation}
	
    From (17.15) in the text, we have 
	
    \begin{equation}
		w_{12}^T\theta_{12} + w_{22}\theta_{22} = 1.\non
	\end{equation}
	
    Plug $\eqref{eq:17-6a}$ into it, we get
	
    \begin{equation}
		-w_{12}^T \bb{W}^{-1}_{11}w_{12}\theta_{22} + w_{22}\theta_{22} = 1,\non
	\end{equation}
	
    which gives
	
    \begin{equation}
		\theta_{22} = 1/(w_{22}-w_{12}^T\bb{W}_{11}^{-1}w_{12}).\non
	\end{equation}
	
    The rest follows directly from $\hat\beta = \bb{W}_11^{-1}w_{12}$.
