---
title: Ex. 12.2
linktitle: Ex 12.2
type: book
date: "2021-01-02T00:00:00+01:00"
# Prev/next pager order (if `docs_section_pager` enabled in `params.toml`)
weight: 1
toc: false
---

???+ question "Ex. 12.2"
	Show that the solution to (12.29) is the same as the solution to (12.25) for a particular kernel.

??? done "Soln. 12.2"
	Define the kernel $K$ by $K(x,y) := h(x)^Th(y)$ for any $x, y\in \mathbb{R}^p$. 
    
    Let $\beta = \sum_{i=1}^N\alpha_ih(x_i)$, then (12.28) in the text reduces to
	
    \begin{eqnarray}
	    f(x) &=& \beta_0 + \sum_{i=1}^N\alpha_ih(x)^Th(x_i)\non\\
	    &=&\beta_0 + h(x)^T\sum_{i=1}^N\alpha_ih(x_i)\non\\
	    &=&\beta_0 + h(x)^T\beta.\non
	\end{eqnarray}
	
    Further note that
	
    \begin{eqnarray}
	    \|\beta\|^2 &=& \beta^T\beta\non\\
	    &=&\left(\sum_{i=1}^N\alpha_ih(x_i)\right)^T\left(\sum_{i=1}^N\alpha_ih(x_i)\right)\non\\
	    &=&\sum_{i=1}^N\sum_{j=1}^N\alpha_i\alpha_jK(x_i, x_j)\non\\
	    &=&\alpha^TK\alpha.\non
	\end{eqnarray}
	
    Therefore, the solution to (12.29) is the same as the solution to (12.25).
