---
title: Ex. 8.4
linktitle: Ex 8.4
type: book
date: "2021-01-02T00:00:00+01:00"
# Prev/next pager order (if `docs_section_pager` enabled in `params.toml`)
weight: 1
toc: false
---

???+ question "Ex. 8.4"
    Consider the bagging method of Section 8.7. Let our estimate $\hat f(x)$ be the $B$-spline smoother $\hat \mu(x)$ of Section 8.2.1. Consider the parametric bootstrap of equation (8.6), applied to this estimator. Show that if we bag $\hat f(x)$, using the parametric bootstrap to generate the bootstrap samples, the bagging estimate $\hat f_{\text{bag}}(x)$ converges to the original estimate $\hat f(x)$ as $B\ra\infty$.

??? done "Soln. 8.4"
    By definition of bagging we get
	
    \begin{equation}
	\label{eq:ex8-4bag}
		\hat f_{\text{bag}}(x) = \frac{1}{B}\sum_{b=1}^B\hat f^\ast_b(x)
	\end{equation}
	
    where 
	
    \begin{equation}
		\hat f^\ast_b(x) = Sy^\ast = S(\hat f(x) + \epsilon_b)\non
	\end{equation}
	
    \begin{equation}
		S = N(N^TN)^{-1}N^T\non
	\end{equation}
	
    and $\epsilon_b\sim N(0,\sigma^2)$ for $B$-spline smoother. Note that $S^2 = S$, we obtain
	
    \begin{equation}
		\hat f^\ast_b(x) = S(\hat f(x) + \epsilon_b) = S(Sy+\epsilon_b) = Sy + S\epsilon_b.\non
	\end{equation}

	Therefore $\eqref{eq:ex8-4bag}$ reduces to
	
    \begin{equation}
		\hat f_{\text{bag}}(x) = Sy + S\left(\frac{1}{B}\sum_{b=1}^B\epsilon_b\right).\non
	\end{equation}
	
    From here it's easy to see that
	
    \begin{equation}
		\lim_{B\ra\infty} \hat f_{\text{bag}}(x) = Sy = \hat f(x).\non 
	\end{equation}