---
title: Ex. 5.7
linktitle: Ex 5.7
type: book
date: "2021-01-02T00:00:00+01:00"
# Prev/next pager order (if `docs_section_pager` enabled in `params.toml`)
weight: 1
toc: false
---

???+ question "Ex. 5.7"
    *Derivation of smoothing splines* ([Nonparametric Regression and Generalized Linear Models](https://www.routledge.com/Nonparametric-Regression-and-Generalized-Linear-Models-A-roughness-penalty/Green-Silverman/p/book/9780412300400)). Suppose that $N\ge 2$, and that $g$ is the natural cubic spline interpolant to the pairs ${x_i, z_i}_1^N$, with $a<x_1<\dots<x_N<b$. This is a natural spline with a knot at every $x_i$; being an $N$-dimensional space of functions, we can determine the coefficients such that it interpolates the sequence $z_i$ exactly. Let $\tilde g$ be any other differentiable function on $[a,b]$ that interpolates the $N$ pairs.
    ???+ question "(a)"
	    Let $h(x) = \tilde g(x) - g(x)$. Use integration by parts and the fact that $g$ is a natural cubic spline to show that
	    
        \begin{eqnarray}
	    \int_a^bg''(x)h''(x)dx &=& -\sum_{j=1}^{N-1}g'''(x_j^+)\{h(x_{j+1}-h(x_j))\}\non\\
	    &=&0.\non
	    \end{eqnarray}
	
    ???+ question "(b)"
        Hence show that
	    
        \begin{equation}
		    \int_a^b\tilde g''(t)^2dt\ge \int_a^bg''(x)^2dt,\non
	    \end{equation}
	    
        and the equality can only hold if $h$ is identically zero in $[a,b]$.
	
    ???+ question "(c)"
        Consider the penalized least squares problem
	    
        \begin{equation}
		    \min_f \left[\sum_{i=1}^N(y_i-f(x_i))^2 + \lambda\int_a^bf''(t)^2dt\right].\non
	    \end{equation}
	    
        Use (b) to argue that the minimizer must be a cubic spline with knots at each of the $x_i$.

??? done "Soln. 5.7"
    ??? done "(a)"
        Using integration by parts, we obtain
        
        \begin{eqnarray}
        \int_a^bg''(x)h''(x)dx &=& [h'(b)g''(b)-h'(a)g''(a)] - \int_a^bg'''(x)h'(x)dx\non\\
        &=&0-\int_a^bg'''(x)h'(x)dx\non\\
        &=&-\int_{x_1}^{x_N}g'''(x)h'(x)dx,\non
        \end{eqnarray}
        
        where the second equation and the last equation follow from the fact that $g$ is a natural cubic spline thus linear on $[a, x_1]$ and $[x_N, b]$. Again, since $g$ is a natural cubic spline, so that $g'''$ is a constant on each interval $(x_j, x_{j+1})$ for $j=1,...,N-1$. By definition of integration we obtain the item above is equal to 
        
        \begin{equation}
            -\sum_{j=1}^{N-1}g'''(x_j^+)\{h(x_{j+1})-h(x_j)\}.\non
        \end{equation}
        
        Since both $\tilde g$ and $g$ interpolate the $N$ pairs $\{x_i, z_i\}_1^N$, we know $h(x_j)=0$ for $j=1,...,N$. Thus the proof is complete.
    ??? done "(b)" 
        From (a), we have
        
        \begin{equation}
            \int_a^bg''(t)h''(t)dt = \int_a^bg''(t)(\tilde g''(t)-g''(t))dt = 0\non
        \end{equation}
        
        so that
        
        \begin{equation}
        \label{eq:57tmp}
            \int_a^bg''(t)^2dt = \int_a^b\tilde g''(t)g''(t)dt.\non
        \end{equation}
        
        Then, we start with $\int_a^b h''(t)^2dt\ge 0$.
        
        \begin{eqnarray}
            \int_a^b h''(t)^2dt &=& \int_a^b (\tilde g''(t)-g''(t))^2dt\non\\
            &=&\int_a^b [\tilde g''(t)^2 + g''(t)^2 - 2\tilde g''(t)g''(t)]dt\non\\
            &=&\int_a^b [\tilde g''(t)^2 + g''(t)^2 - 2g''(t)^2]dt\non\\
            &=&\int_a^b [\tilde g''(t)^2 - g''(t)^2]dt\non\\
            &\ge&0. \non
        \end{eqnarray}
        
        Thus we have
        
        \begin{equation}
            \int_a^b\tilde g''(t)^2dt \ge \int_a^bg''(t)^2dt,\non
        \end{equation}
        
        and the equality can only hole if $h''$ is zero in $[a,b]$. Thus $h$ is linear in $[a,b]$. However by definition $h(x_j)=0$ for all $j=1, ..., N$, we conclude that $h$ must be identically zero in $[a,b]$. 
    
    ??? done "(c)" 
        Consider a minimizer $f_0$. We can always construct a natural cubic spline $f$ such that $f_0$ and $f$ have the same values at each of $\{x_i, i=1,...,N\}$, therefor we have $\sum_{i=1}^N(y_i-f_0(x_i))^2 = \sum_{i=1}^N(y_i-f(x_i))^2$. From (b) we know that
        
        \begin{equation}
            \int_a^b f_0''(t)^2dt \ge \int_a^b f''(t)^2dt.\non
        \end{equation}
        
        Since $f_0$ is a minimize, the above inequality is actually a equality, therefore by (b) again, $f_0=f$ in $[a, b]$. The proof is complete. 
    