---
title: Ex. 5.16
linktitle: Ex 5.16
type: book
date: "2021-01-02T00:00:00+01:00"
# Prev/next pager order (if `docs_section_pager` enabled in `params.toml`)
weight: 1
toc: false
---

???+ question "Ex. 5.16"
    Consider the ridge regression problem (5.53), and assume $M\ge N$. Assume you have a kernel $K$ that computes the inner product $K(x,y) = \sum_{m=1}^Mh_m(x)h_m(y)$.
	
    ???+ question "(a)"
	    Derive (5.62) on page 171 in the text. How would you compute the matrices $\bb{V}$ and $\bb{D}_\gamma$, given $K$? Hence show that (5.63) is equivalent to (5.53).
	???+ question "(b)" 
        Show that
	    
        \begin{eqnarray}
	     \hat{\mathbf{f}} &=& \bb{H}\hat\beta\non\\
	     &=&\bb{K}(\bb{K} + \lambda\bb{I})^{-1}\bb{y},\non
	    \end{eqnarray} 
	    
        where $\bb{H}$ is the $N\times M$ matrix of evaluations $h_m(x_i)$, and $\bb{K} = \bb{H}\bb{H}^T$ the $N\times N$ matrix of inner-product $h(x_i)^Th(x_j)$.
	???+ question "(c)" 
        Show that 
	    
        \begin{eqnarray}
	     \hat f(x) &=& h(x)^T\hat{\bm{\beta}}\non\\
	     &=& \sum_{i=1}^NK(x, x_i)\hat{\bm{\alpha}_i}\non
	    \end{eqnarray}
	    
        and $\hat{\bm{\alpha}} = (\bb{K} + \lambda \bb{I})^{-1}\bb{y}$.
	???+ question "(d)" 
        How would you modify your solution if $M < N$?


??? done "Soln. 5.16"
    ??? done "(a)"
        By definition of the kernel $K$, we have
		
        \begin{equation}
			K(x, y) = \sum_{m=1}^Mh_m(x)h_m(y) = \sum_{i=1}^\infty \gamma_i\phi_i(x)\phi_i(y).\non
		\end{equation}
		
        Multiply each summand above by $\phi_k(x)$ and calculate $\langle K(x,y), \phi_k(x) \rl$,
		
        \begin{equation}
		\label{eq:5-16a}
			\sum_{m=1}^M\langle h_m(x), \phi_k(x)\rl h_m(y) = \sum_{i=1}^\infty \langle \phi_i(x), \phi_k(x)\rl \phi_i(y).
		\end{equation}
		
        Since $\{\phi_i, i=1,...,\infty\}$ are orthogonal, we have 
		
        \begin{equation}
			\langle \phi_i(x), \phi_k(x) \rl = \begin{cases}
				1 & \text{ if } i=k,\\
				0 & \text{ otherwise.}
			\end{cases}\non
		\end{equation}
		
        Thus, $\eqref{eq:5-16a}$ becomes
		
        \begin{equation}
			\sum_{m=1}^M\langle h_m(x), \phi_k(x)\rl h_m(y) = \gamma_k\phi_k(y).\non
		\end{equation}

		Let $g_{km} = \langle h_m(x), \phi_k(x) \rl$ and calculate $\langle K(x,y), \phi_l(y) \rl$, we get
		
        \begin{eqnarray}
		    \sum_{m=1}^M g_{km}h_m(y) &=& \gamma_k\phi_k(y),\non\\
		    \sum_{m=1}^M g_{km} \langle h_m(y), \phi_l(y) \rl &=& \gamma_k \langle \phi_k(y), \phi_l(y) \rl ,\non\\
		    \sum_{m=1}^M g_{km}g_{lm} &=& \gamma_k\delta_{k,l}\non
		\end{eqnarray}
		
        where $\delta_{k,l} = 1$ if $k=l$ and 0 otherwise. 

		Let $\bb{G}_M = \{g_{nm}\} \in \mathbb{R}^{M\times N}$, we have
		
        \begin{equation}
			\bb{G}_M\bb{G}_M^T = \text{diag}\{\gamma_1,\gamma_2,...,\gamma_M\} = \bb{D}_\gamma.\non
		\end{equation}
		
        Let $\bb{V}^T = \bb{D}_\gamma^{-\frac{1}{2}}\bb{G}_M$, we have
		
        \begin{equation}
			\bb{V}\bb{V}^T\bb{G}_M^T = \bb{G}_M^T\bb{D}_\gamma^{-1}\bb{G}_M = \bb{I}_N.\non
		\end{equation}
		
        Let $h(x) = (h_1(x), h_2(x), ..., h_M(x))^T$ and $\phi(x) = (\phi_1(x), \phi_2(x), ..., \phi_M(x))^T$, then the three equations above can be rewritten as 
		
        \begin{eqnarray}
		    \bb{G}_Mh(x) &=& \bb{D}_\gamma\phi(x)\non\\
		    \bb{V}\bb{D}^{-\frac{1}{2}}_\gamma\bb{G}_Mh(x) &=& \bb{V}\bb{D}^{-\frac{1}{2}}_\gamma\bb{D}_\gamma\phi(x)\non\\
		    h(x) &=&\bb{V}\bb{D}^{\frac{1}{2}}_\gamma.\non
		\end{eqnarray}
		
        To show that (5.63) is equivalent to (5.53) in the text, we start with (5.63). Let $\beta = (\beta_1, \beta_2,...,\beta_m)^T$ and $c=\bb{D}_\gamma^{\frac{1}{2}}\bb{V}^T\beta$,
		
        \begin{eqnarray}
		 && \min_{\{\beta_m\}_1^M}\sum_{i=1}^N\left(y_i-\sum_{m=1}^M\beta_mh_m(x_i)\right)^2 + \lambda \sum_{m=1}^M\beta_m^2\non\\
		 &=&\min_{\beta}\sum_{i=1}^N(y_i-\beta^Th(x_i))^2 + \lambda\beta^T\beta\non\\
		 &=&\min_{\beta} \sum_{i=1}^N(y_i-\beta^T\bb{V}\bb{D}^{\frac{1}{2}}_\gamma\phi(x_i))^2 + \lambda\beta^T\beta\non\\
		 &=&\min_{c}\sum_{i=1}^N(y_i-c^T\phi(x_i))^2 + \lambda (\bb{V}\bb{D}^{\frac{1}{2}}_\gamma c)^T \bb{V}\bb{D}^{\frac{1}{2}}_\gamma c\non\\
		 &=&\min_{c}\sum_{i=1}^N(y_i-c^T\phi(x_i))^2 + \lambda c^Tc\bb{D}_\gamma^{-1}\non\\
		 &=&\min_{\{c_j\}_1^\infty}\sum_{i=1}^N\left(y_i-\sum_{j=1}^\infty c_j\phi_j(x_i)\right)^2 + \lambda \sum_{j=1}^\infty \frac{c_j^2}{\gamma_j},\non
		\end{eqnarray}
		
        which is (5.53) in the text.

    ??? done "(b)"
        Recall that in (a) we have
		
        \begin{equation}
		 	\min_{\beta}\sum_{i=1}^N(y_i-\beta^Th(x_i))^2 + \lambda\beta^T\beta.\non
		\end{equation} 
		
        Taking derivative w.r.t $\beta$ and setting it to be zero yields
		
        \begin{equation}
		 	-\bb{H}^T(\by-\bb{H}\hat\beta) + \lambda \hat\beta = 0.\non
		\end{equation}
		
        Thus we have
		
        \begin{equation}
		 	\hat\beta = (\bb{H}^T\bb{H} + \lambda \bb{I})^{-1}\bb{H}^T\by\non
		 \end{equation}
		
        and 
		
        \begin{equation}
		 	\hat{\mathbf{f}} = \bb{H}(\bb{H}^T\bb{H} + \lambda \bb{I})^{-1}\bb{H}^T\by.\non
		\end{equation}
		
        By Woodbury matrix identity, we have
		
        \begin{eqnarray}
		     (\bb{H}^T\bb{H} + \lambda \bb{I})^{-1} &=& \frac{1}{\lambda}\bb{I} - \frac{1}{\lambda}\bb{I}\bb{H}^T\left(\bb{I} + \frac{1}{\lambda}\bb{H}\bb{H}^T\right)^{-1}\bb{H}\cdot\frac{1}{\lambda}\bb{I}\non.
		\end{eqnarray}
		
        Therefore, we have
		
        \begin{eqnarray}
		     \hat{\mathbf{f}} &=& \frac{1}{\lambda}\bb{H}\bb{H}^T\by - \frac{1}{\lambda}\bb{H}\bb{H}^T\left(\lambda\bb{I}+\bb{H}\bb{H}^T\right)^{-1}\bb{H}\bb{H}^T\by\non\\
		     &=&\frac{1}{\lambda}\bb{H}\bb{H}^T\left[\bb{I}-(\lambda\bb{I}+\bb{H}\bb{H}^T)^{-1}\bb{H}\bb{H}^T\right]\by\non\\
		     &=&\frac{1}{\lambda}\bb{H}\bb{H}^T\left[(\lambda\bb{I}+\bb{H}\bb{H}^T)^{-1}(\lambda\bb{I}+\bb{H}\bb{H}^T)-(\lambda\bb{I}+\bb{H}\bb{H}^T)^{-1}\bb{H}\bb{H}^T\right]\by\non\\
		     &=&\frac{1}{\lambda}\bb{H}\bb{H}^T\left[(\lambda\bb{I}+\bb{H}\bb{H}^T)^{-1}\lambda\bb{I}\right]\by\non\\
		     &=&\bb{H}\bb{H}^T(\lambda\bb{I}+\bb{H}\bb{H}^T)^{-1}\by\non\\
		     &=&\bb{K}(\bb{K}+\lambda\bb{I})^{-1}\by.\non
		\end{eqnarray}

    ??? done "(c)" 
        This is directly derived from (b).

    ??? done "(d)"
        The solution remains the same as $\bb{K}+\lambda\bb{I}$ is invertible as long as $\lambda \neq 0$. When $\lambda = 0$ however, we have 
		
        \begin{equation}
		 	\hat{\mathbf{f}} = \bb{H}\hat\beta = \bb{H}(\bb{H}^T\bb{H})^{-1}\bb{H}^T\by = \by.\non
		\end{equation}