---
title: Ex. 5.14
linktitle: Ex 5.14
type: book
date: "2021-01-02T00:00:00+01:00"
# Prev/next pager order (if `docs_section_pager` enabled in `params.toml`)
weight: 1
toc: false
---

???+ question "Ex. 5.14"
    Derive the constraints on the $\alpha_j$ in the thin-plate spline expansion (5.39) to guarantee that the penalty $J(f)$ is finite. How else could one ensure that the penalty was finite?

??? done "Soln. 5.14"
    Consider 

	\begin{equation}
		f(x,y) = \beta_0 + \beta^T(x,y) + \sum_{j=1}^N\alpha_jh_j(x,y)\non
	\end{equation}
	
    where
	
    \begin{eqnarray}
		h_j(x,y) &=& [(x-x_j)^2 + (y-y_j)^2]\log\left(\sqrt{(x-x_j)^2 + (y-y_j)^2}\right)\non\\
		&=&\frac{1}{2}[(x-x_j)^2 + (y-y_j)^2]\log((x-x_j)^2 + (y-y_j)^2).\non
	\end{eqnarray}
	
    Without loss of generality, we will drop the constant and linear term $\beta_0 + \beta^T(x,y)$ in $f$ since they vanish after taking second derivatives below.

	The penalty function $J$ is
	
    \begin{equation}
		J(f) = \int\int_{\mathbb{R}^2}\left[\left(\frac{\partial^2f(x,y)}{\partial x^2}\right)^2+2\left(\frac{\partial^2f(x,y)}{\partial x\partial y}\right)^2 + \left(\frac{\partial^2f(x,y)}{\partial y^2}\right)^2\right]dxdy.\non
	\end{equation}

	Next we compute each integrand above. First, denote 
	
    \begin{eqnarray}
		r_{jx} &=& x-x_j\non\\
		r_{jy} &=& y-y_j\non\\
	    r^2_j &=& r^2_{jx} + r^2_{jy}=(x-x_j)^2 + (y-y_j)^2.\non 
	\end{eqnarray}
	
    Then we have
	
    \begin{eqnarray}
	    \frac{\partial f(x,y)}{\partial x} &=& \sum_{j=1}^N\alpha_j[r_{jx}(\log(r_j^2) + 1)]\non\\
	    \frac{\partial^2 f(x,y)}{\partial^2 x} &=& \sum_{j=1}^N\alpha_j\left[\log(r_j^2) + 2\frac{r_{jx}^2}{r_j^2} + 1\right]\non\\
	    \frac{\partial^2 f(x,y)}{\partial x\partial y} &=& \sum_{j=1}^N\alpha_j\frac{2r_{jx}r_{jy}}{r_j^2}\non\\
	    \frac{\partial^2 f(x,y)}{\partial^2 y} &=& \sum_{j=1}^N\alpha_j\left[\log(r_j^2) + 2\frac{r_{jy}^2}{r_j^2} + 1\right].\non	    
	\end{eqnarray}

	To get penalty $J[f]$, we calculate the first integrand as
	
    \begin{eqnarray}
		&&\left(\frac{\partial^2 f(x,y)}{\partial^2 x}\right)^2\non\\
		&=&\left(\sum_{j=1}^N\alpha_j\log(r_j^2)\right)^2 + \left(\sum_{j=1}^N2\alpha_j\frac{r_{jx}^2}{r_j^2}\right)^2 + \left(\sum_{j=1}^N\alpha_j\right)^2\non\\
		&&+2\left(\sum_{j=1}^N\alpha_j\log(r_j^2)\right)\left(\sum_{j=1}^N2\alpha_j\frac{r_{jx}^2}{r_j^2}\right)\non\\
		&&+2\left(\sum_{j=1}^N\alpha_j\log(r_j^2)\right)\left(\sum_{j=1}^N\alpha_j\right)\non\\
		&&+2\left(\sum_{j=1}^N2\alpha_j\frac{r_{jx}^2}{r_j^2}\right)\left(\sum_{j=1}^N\alpha_j\right).\non
	\end{eqnarray}
	
    At this point we see that $\sum_{j=1}^N\alpha_j = 0$, otherwise the integral would be infinite. So that above integrand is simplified to
	
    \begin{eqnarray}
	\label{eq:5-14a}
	    &&\left(\frac{\partial^2 f(x,y)}{\partial^2 x}\right)^2\non\\
	    &=&\left(\sum_{j=1}^N\alpha_j\log(r_j^2)\right)^2 + \left(\sum_{j=1}^N2\alpha_j\frac{r_{jx}^2}{r_j^2}\right)^2+2\left(\sum_{j=1}^N\alpha_j\log(r_j^2)\right)\left(\sum_{j=1}^N2\alpha_j\frac{r_{jx}^2}{r_j^2}\right).\non
	\end{eqnarray}
	
    Similarly we have
	
    \begin{eqnarray}
	\label{eq:5-14b}
	    \left(\frac{\partial^2 f(x,y)}{\partial x\partial y}\right)^2=\left(\sum_{j=1}^N\alpha_j\frac{2r_{jx}r_{jy}}{r_j^2}\right)^2.\non
	\end{eqnarray}
	
    and
	
    \begin{eqnarray}
	\label{eq:5-14c}
	    &&\left(\frac{\partial^2 f(x,y)}{\partial^2 y}\right)^2\non\\
	    &=&\left(\sum_{j=1}^N\alpha_j\log(r_j^2)\right)^2 + \left(\sum_{j=1}^N2\alpha_j\frac{r_{jy}^2}{r_j^2}\right)^2+2\left(\sum_{j=1}^N\alpha_j\log(r_j^2)\right)\left(\sum_{j=1}^N2\alpha_j\frac{r_{jy}^2}{r_j^2}\right).\non
	\end{eqnarray}
	
    Sum them up we get
	
    \begin{eqnarray}
	    &&2\left(\sum_{j=1}^N\alpha_j\log(r_j^2)\right)^2 + \left(\sum_{j=1}^N2\alpha_j\frac{r_{jx}^2}{r_j^2}\right)^2+\left(\sum_{j=1}^N2\alpha_j\frac{r_{jy}^2}{r_j^2}\right)^2\non\\
	    && + \left(\sum_{j=1}^N\alpha_j\frac{2r_{jx}r_{jy}}{r_j^2}\right)^2\non\\
	    && + 2\left(\sum_{j=1}^N\alpha_j\log(r_j^2)\right)\left(\sum_{j=1}^N2\alpha_j\frac{r_{jx}^2+r_{jy}^2}{r_j^2}\right).\non
	\end{eqnarray}
	
    Note that $\frac{r_{jx}^2+r_{jy}^2}{r_j^2}=1$ and $\sum_{j=1}^N\alpha_j=0$, the last summand above vanishes and we are left with
	
    \begin{equation}
		\left(\sum_{j=1}^N\alpha_j\log(r_j^2)\right)^2 + \left(\sum_{j=1}^N2\alpha_j\frac{r_{jx}^2}{r_j^2}\right)^2+\left(\sum_{j=1}^N2\alpha_j\frac{r_{jy}^2}{r_j^2}\right)^2+ \left(\sum_{j=1}^N\alpha_j\frac{2r_{jx}r_{jy}}{r_j^2}\right)^2.\non
	\end{equation}
	
    !!! note "Remark"
        It has been shown that $\sum_{j=1}^N\alpha_jx_j=0$ (see, e.g., \cite{david1996}) , however I don't see how to arrive that from here.