---
title: Ex. 14.23
linktitle: Ex 14.23
type: book
date: "2021-01-02T00:00:00+01:00"
# Prev/next pager order (if `docs_section_pager` enabled in `params.toml`)
weight: 1
toc: false
---

???+ question "Ex. 14.23"
	*Algorithm for non-negative matrix factorization* (Wu and Lange, 2007). A function $g(x, y)$ is said to *minorize* a function $f(x)$ if 

	\begin{equation}
		g(x, y) \le f(x), \  g(x,x) = f(x)\non
	\end{equation}
	
    for all $x, y$ in the domain. This is useful for maximizing $f(x)$ since it is easy to show that $f(x)$ is nondecreasing under the update 
	
    \begin{equation}
		x^{s+1} = \underset{x}{\operatorname{argmax}} g(x,x^s).\non
	\end{equation}
	
    There are analogous definitions for *majorization*, for minimizing a function $f(x)$. The resulting algorithms are known as *MM* algorithms, for minorize-maximize or majorize-minimize (Lange, 2004). It also can be shown that the EM algorithm (8.5) is an example of an MM algorithm: see Section 8.5.3 and Exercise [8.2](../8-Model-Inference-and-Averaging/ex8-2.md) for details.

	(a) Consider maximization of the function $L(\bb{W}, \bb{H})$ in (14.73), written here without the matrix notation

    \begin{equation}
        L(\bb{W}, \bb{H}) = \sum_{i=1}^N\sum_{j=1}^p\left[x_{ij}\log\left(\sum_{k=1}^rw_{ik}h_{kj}\right)-\sum_{k=1}^rw_{ik}h_{kj}\right].\non
    \end{equation}
    
    Using the concavity of $\log(x)$, show that for any set of $r$ values $y_k\ge 0$ and $0\le c_k \le 1$ with $\sum_{k=1}^r c_k = 1$,
    
    \begin{equation}
        \log\left(\sum_{k=1}^r y_k\right)\ge \sum_{k=1}^r c_k \log(y_k/c_k).\non
    \end{equation}
    
    Hence 
    
    \begin{equation}
        \log\left(\sum_{k=1}^r w_{ik}h_{kj}\right)\ge \sum_{k=1}^r\frac{a^s_{ikj}}{b^s_{ij}}\log\left(\frac{b^s_{ij}}{a^s_{ikj}}w_{ik}h_{kj}\right),\non
    \end{equation}
    
    where 
    
    \begin{equation}
        a^s_{ikj} = w^s_{ik}h^s_{kj} \ \text{and} \ b^s_{ij} = \sum_{k=1}^rw_{ik}^sh^s_{kj},\non
    \end{equation}
    
    and $s$ indicates the current iteration.
		
    (b) Hence show that, ignoring constants, the function
	
    \begin{eqnarray}
        g(\bW, \bb{H}|\bW^s, \bb{H}^s) &=& \sum_{i=1}^N\sum_{j=1}^p\sum_{k=1}^rx_{ij}\frac{a^s_{ikj}}{b^s_{ij}}\left(\log w_{ik} + \log h_{kj}\right)\non\\
        &&\ \ \ \ - \sum_{i=1}^N\sum_{j=1}^p\sum_{k=1}^rw_{ik}h_{kj}\non
    \end{eqnarray}
    
    minorizes $L(\bW, \bb{H})$.
    
    (c) Set the partial derivatives of $g(\bW, \bb{H}|\bW^s, \bb{H}^s)$ to zero and hence derive the updating steps (14.74).

??? done "Soln. 14.20"
	(a) Suppose that $f(x)$ is convex, then we claim 
	
    \begin{equation}
	\label{eq:14-23a}
		f\left(\sum_{i=1}^nc_ix_i\right) \le \sum_{i=1}^nc_if(x_i),
	\end{equation}
	
    where $\sum_{i=1}^nc_i = 1$ and $c_i\ge 0$ for $i=1,...,n$. To prove it, we use mathematical induction. By definition, we know that $\eqref{eq:14-23a}$ holds when $n=2$. Suppose $n > 2$, assume that $0 < c_n < 1$ and denote $c_0 = 1-c_n > 0$ and $x_0 = \sum_{i=1}^{n-1}c_ix_i/c_0$.
	
	Then we have 
	
    \begin{eqnarray}
		f\left(\sum_{i=1}^nc_ix_i\right) &=& f\left(\sum_{i=1}^{n-1}c_ix_i + c_n x_n\right)\non\\
		&=&f(c_0x_0 + c_nx_n)\non\\
		&\le& c_0f(x_0) + c_nf(x_n)\non\\
		&=&c_0 f\left(\sum_{i=1}^{n-1}c_ix_i/c_0\right) + c_nf(x_n)\non\\
		&\le& c_0 \frac{1}{c_0}\sum_{i=1}^{n-1}c_if(x_i) + c_n f(x_n)\non\\
		&=&\sum_{i=1}^nc_if(x_i),\non
	\end{eqnarray}
	
    which is $\eqref{eq:14-23a}$.

	For concave function $f$, we have 
	
    \begin{equation}
		f\left(\sum_{i=1}^nc_ix_i\right) \ge \sum_{i=1}^nc_if(x_i).\non
	\end{equation}
	
    Therefore we know the claim in (a) is correct.

	(b) We only need focus on the first term. 
	
	Note that
	
    \begin{eqnarray}
		g(\bW, \bb{H}|\bW^s, \bb{H}^s) &=& \sum_{i=1}^N\sum_{j=1}^p\sum_{k=1}^rx_{ij}\frac{a^s_{ikj}}{b^s_{ij}}\left(\log w_{ik} + \log h_{kj}\right)\non\\
		&=&\sum_{i=1}^N\sum_{j=1}^p\sum_{k=1}^rx_{ij}\frac{a^s_{ikj}}{b^s_{ij}}\log \left(\frac{b^s_{ij}}{a^s_{ikj}}w_{ik}h_{kj}\right)- C,\non
	\end{eqnarray}
	
    where the constant $C$ (independent of $\bW$ and $\bb{H}$) is 
	
    \begin{equation}
		C = \sum_{i=1}^N\sum_{j=1}^p\sum_{k=1}^rx_{ij}\frac{a^s_{ikj}}{b^s_{ij}}\log \frac{b^s_{ij}}{a^s_{ikj}}.\non
	\end{equation}

	Therefore, by (a), we have 
	
    \begin{equation}
		g(\bW, \bb{H}|\bW^s, \bb{H}^s) \le L(\bb{W}, \bb{H}),\non
	\end{equation}
	
    and it's easy to verify that the equation holds when $\bW^s = \bW$ and $\bb{H}^s = \bb{H}$.
	
	(c) Fix $i$ and $k$, we have 
	
    \begin{eqnarray}
		\frac{\partial g(\bW, \bb{H}|\bW^s, \bb{H}^s)}{\partial w_{ik}} &=& \sum_{j=1}^p x_{ij}\frac{a^s_{ikj}}{b^s_{ij}}\frac{1}{w_{ik}} - \sum_{j=1}^ph_{kj}\non\\
		&=&0,\non 
	\end{eqnarray}
	
    so that 
	
    \begin{eqnarray}
		w_{ik} &=& \frac{\sum_{j=1}^px_{ij}\frac{a^s_{ikj}}{b^s_{ij}}}{\sum_{j=1}^ph_{kj}}\non\\
		&=&\left(\sum_{j=1}^px_{ij} \frac{w^s_{ik}h^s_{kj}}{\sum_{k'=1}^rw^s_{ik'}h^s_{k'j}}\right)\Bigg/\sum_{j=1}^ph_{kj}\non\\
		&=&w_{ik}^s\frac{\sum_{j=1}^ph_{kj}x_{ij}/(\bW\bb{H})_{ij}}{\sum_{j=1}^ph_{kj}},\non
	\end{eqnarray}
	
    which is (14.74) in the text. The same arguments apply to the update of $h_{kj}$, thus we omit it for brevity.